added actual backwards chaining

ModularEngine/src/LogicEngine.FStar/coredkal.fst
@@ -25,13 +25,13 @@ module CoreDKAL
 (********************)
 
 open Types
-  
+
 (** only for Core DKAL **)
 type infostrate = list term
 type substrate
 type varDecl = list var
 type prefix = list term
-  
+
 (*************)
 (* Utilities *)
 (*************)
@@ -49,8 +49,8 @@ let rec mem (a : 'a) (l: list 'a) : option (Mem 'a a l) =
   | h::t when h=a -> Some(Mem_hd a t)
   | h::t -> (match mem a t with
                | None -> None
-			   | Some(m) -> Some(Mem_tl a h t m))
-  
+               | Some(m) -> Some(Mem_tl a h t m))
+
 val memInfostrate : i:term -> is:infostrate -> option (Mem i is)
 let memInfostrate i _I = mem i _I
 
@@ -59,12 +59,12 @@ let memInfostrate i _I = mem i _I
 (* MkPrefix [p1;...;pn] i (p1 said (p2 said ... (pn said i))) *)
 type MkPrefix :: list term => term => term => P =
   | MkPrefix_Nil : i:term -> MkPrefix [] i i
-  | MkPrefix_Cons : p:term -> ps:list term -> i:term -> i':term 
+  | MkPrefix_Cons : p:term -> ps:list term -> i:term -> i':term
                    -> MkPrefix ps i i'
                    -> MkPrefix (p::ps) i (App SaidInfon [p; i'])
-				   (* Rk: cannot use said here *)
+                   (* Rk: cannot use said here *)
 
-(* Intuition:                                                    *) 
+(* Intuition:                                                    *)
 (* mkPrefix [p1;...;pn] i = ( (p1 said (... pn said i)), proof ) *)
 val mkPrefix: pref:prefix -> i:term -> (i':term * dummy:(MkPrefix pref i i'){pref=[] => i=i'})
 let rec mkPrefix pref i =
@@ -77,12 +77,12 @@ let rec mkPrefix pref i =
 val func_typing : func -> option ((list typ) * typ)
 let func_typing = function
  (* could also take code from Ast.Infon/Primitives.fs *)
-  | SeqRule -> None (*[RuleT; RuleT], RuleT*) 
+  | SeqRule -> None (*[RuleT; RuleT], RuleT*)
                     (* any number of args possible *)
   | EmptyRule -> Some([], RuleT)
   | Rule -> Some([Condition; Action], RuleT)
   | RuleOnce -> Some([Condition; Action], RuleT)
-  | SeqCondition -> None (*[Condition; Condition], Condition*) 
+  | SeqCondition -> None (*[Condition; Condition], Condition*)
                          (* any number of args possible *)
   | EmptyCondition -> Some([], Condition)
   | WireCondition -> Some([Infon; Principal], Condition)
@@ -113,10 +113,22 @@ let func_typing = function
                         (* any number of args possible *)
   | AsInfonEvidence -> Some([SubstrateQuery], Evidence)
   | RelationInfon r -> Some(r.argsType, r.retType)
-				 
+
+
+val fold_left_dep : res:'a -> l:list 'b -> ('a -> x:'b -> Mem x l -> 'a) -> 'a
+let rec fold_left_dep res l f = match l with
+  | [] -> res
+  | h::t -> fold_left_dep (f res h (Mem_hd h t)) t
+                          (fun res x m -> f res x (Mem_tl x h t m))
+
+val collect_dep : l:list 'a -> (x:'a -> Mem x l -> list 'b) -> list 'b
+let rec collect_dep l f =
+  fold_left_dep [] l (fun res x m -> append res (f x m))
+
+
 (******************************)
 (* Trusted external functions *)
-(******************************) 
+(******************************)
 
 (* 1. Dynamic type tests from .NET *)
 type TypeOf :: object => typ => E
@@ -125,51 +137,51 @@ type TypeOf :: object => typ => E
 (* 2. Queries to external databases i.e., Substrate *)
 type SubstrateSays :: substrate => ISubstrateQueryTerm => E
 (* extern Runtime  FIXME *) val check_substrate : s:substrate -> q:ISubstrateQueryTerm -> b:bool{b=true => SubstrateSays s q}
-
+(*
 
 (***********************)
 (* Inductive judgments *)
-(***********************) 
-
+(***********************)
+*)
 (* could do a cast in an external file *)
-type types :: varDecl => term => typ => P =		   
-  | Types_Var : G:varDecl 
-			   -> v:var
-			   -> Mem v G
+type types :: varDecl => term => typ => P =
+  | Types_Var : G:varDecl
+               -> v:var
+               -> Mem v G
                -> types G (Var v) v.typ
-			   (* TODO: change rules for name clashes/scope *)
+               (* TODO: change rules for name clashes/scope *)
   | Types_ConstTrueT : G:varDecl -> types G (Const TrueT) Boolean
   | Types_ConstFalseT : G:varDecl -> types G (Const FalseT) Boolean
   | Types_ConstPrincipalConstant : G:varDecl -> p:principal
                              -> types G (Const (PrincipalConstant p)) Principal
   | Types_ConstSubstrateConstant : G:varDecl -> t:typ -> o:object{TypeOf o t}
                                  -> types G (Const (SubstrateConstant o)) t
-  | Types_ForallT : G:varDecl -> x:var -> i:term 
+  | Types_ForallT : G:varDecl -> x:var -> i:term
                    -> types (x::G) i Infon
                    -> types G (ForallT x i) Infon
   | Types_AppEmptyInfon : G:varDecl -> types G (App EmptyInfon []) Infon
   | Types_AppSaidInfon : G:varDecl -> p:term -> i:term
                          -> types G p Principal
-						 -> types G i Infon
-						 -> types G (App SaidInfon [p; i]) Infon
+                         -> types G i Infon
+                         -> types G (App SaidInfon [p; i]) Infon
   | Types_AppAsInfon : G:varDecl -> q:ISubstrateQueryTerm
                        -> types G (App AsInfon [(SubstrateQueryTerm q)]) Infon
   | Types_AppAndInfon : G:varDecl -> i:term -> j:term (* TODO: extend to n *)
                      -> types G i Infon
-					 -> types G j Infon 
-					 -> types G (App AndInfon [i; j]) Infon
+                     -> types G j Infon
+                     -> types G (App AndInfon [i; j]) Infon
   | Types_AppImpliesInfon : G:varDecl -> i:term -> j:term
                      -> types G i Infon
-					 -> types G j Infon 
-					 -> types G (App ImpliesInfon [i; j]) Infon
-  | Types_AppJustifiedInfon : G:varDecl -> i:term -> e:term 
+                     -> types G j Infon
+                     -> types G (App ImpliesInfon [i; j]) Infon
+  | Types_AppJustifiedInfon : G:varDecl -> i:term -> e:term
                             -> types G i Infon
-							-> types G e Evidence
-							-> types G (App JustifiedInfon [i; e]) Infon
+                            -> types G e Evidence
+                            -> types G (App JustifiedInfon [i; e]) Infon
   | Types_AppRelationInfon : G:varDecl -> r:relationInfon (* no type check here *)
                            -> l:list term
-						 (* TODO: need to typecheck all the subterms! *)
-						   -> types G (App (RelationInfon r) l) Infon
+                         (* TODO: need to typecheck all the subterms! *)
+                           -> types G (App (RelationInfon r) l) Infon
 
 (* type names = list string *)
 (* type Subst :: (\* binders crossed *\) names => (\* subst into this term *\) term => (\* for this *\) var => (\* with this *\) term => (\* result *\) term => P =  *)
@@ -191,164 +203,164 @@ type types :: varDecl => term => typ => P =
 
 
 (* Subst i x u i'  iff  i[u/x] = i' *)
-type Subst :: term => var => term => term => P = 
+type Subst :: term => var => term => term => P =
   | Subst_VarRepl : x:var -> u:term -> Subst (Var x) x u u
-  | Subst_VarIgnore : y:var -> u:term -> x:var{not(x = y)} 
+  | Subst_VarIgnore : y:var -> u:term -> x:var{not(x = y)}
                     -> Subst (Var y) x u (Var y)
-  | Subst_Const : x:var -> u:term -> c:constant 
+  | Subst_Const : x:var -> u:term -> c:constant
                 -> Subst (Const c) x u (Const c)
-  | Subst_ForallTIgnore : x:var -> i:term -> u:term 
+  | Subst_ForallTIgnore : x:var -> i:term -> u:term
                         -> Subst (ForallT x i) x u (ForallT x i)
-  | Subst_ForallTRepl : y:var -> i:term 
+  | Subst_ForallTRepl : y:var -> i:term
                       -> x:var{not(x = y)}
-                      -> u:term 
-					  -> i' : term
-					  -> Subst i x u i'
-					  -> Subst (ForallT y i) x u (ForallT y i')
+                      -> u:term
+                      -> i' : term
+                      -> Subst i x u i'
+                      -> Subst (ForallT y i) x u (ForallT y i')
   (* TODO: do something more general for App? *)
-  | Subst_App0 : f:func -> x:var -> u:term 
+  | Subst_App0 : f:func -> x:var -> u:term
                -> Subst (App f []) x u (App f [])
-  | Subst_App1 : f:func -> x:var -> u:term 
+  | Subst_App1 : f:func -> x:var -> u:term
                -> i:term -> i':term
-			   -> Subst i x u i'
+               -> Subst i x u i'
                -> Subst (App f [i]) x u (App f [i'])
-  | Subst_App2 : f:func -> x:var -> u:term 
+  | Subst_App2 : f:func -> x:var -> u:term
                -> i:term -> i':term
                -> j:term -> j':term
-			   -> Subst i x u i'
-			   -> Subst j x u j'
+               -> Subst i x u i'
+               -> Subst j x u j'
                -> Subst (App f [i; j]) x u (App f [i'; j'])
   (* try with n *)
   (*| Subst_Appn : f:func -> x:var -> u:term
-               -> ilist : term list 
-			   -> ilist': term list{}
-			   -> Forall i in ilist, Subst i x u i'
-			   -> ... *)
+               -> ilist : term list
+               -> ilist': term list{}
+               -> Forall i in ilist, Subst i x u i'
+               -> ... *)
   (* Is this really true? Any variable ever in the ISubstrateQueryTerm? *)
   | Subst_SubstrateQueryTerm : q:ISubstrateQueryTerm -> x:var -> u:term
                      -> Subst (SubstrateQueryTerm q) x u (SubstrateQueryTerm q)
-						   
-						   
+
+
 type entails :: substrate => infostrate => varDecl => term => P =
   | Entails_Emp : S:substrate -> I:infostrate -> G:varDecl
                -> pref: prefix
-			   -> result: term
-			   -> MkPrefix pref (App EmptyInfon []) result
-			      (* Rk: cannot just use empty in place of App EmptyInfon [] *)
-			   -> entails S I G result
+               -> result: term
+               -> MkPrefix pref (App EmptyInfon []) result
+                  (* Rk: cannot just use empty in place of App EmptyInfon [] *)
+               -> entails S I G result
 
   | Entails_Hyp_Knowledge : S:substrate -> I:infostrate -> G:varDecl
                           -> i:term
                           -> Mem i I
                           -> entails S I G i
-						  
+
   | Entails_Hyp_Substrate : S:substrate -> I:infostrate -> G:varDecl
                           -> q:ISubstrateQueryTerm{SubstrateSays S q}
-						  (* Eventually, we get a signature from the DB about this fact *)
+                          (* Eventually, we get a signature from the DB about this fact *)
                           -> entails S I G (App AsInfon [(SubstrateQueryTerm q)])
-						  (* Rk: need parenthesis inside the list *)
+                          (* Rk: need parenthesis inside the list *)
 
 
   (* Q: here order of G matters; make sure that's all right; I think so *)
   | Entails_Q_Intro : S:substrate -> I:infostrate -> G:varDecl
                     -> x:var -> i:term -> i':term
-					-> result:term
-					-> pref:prefix
-			        -> MkPrefix pref (ForallT x i) result
-					-> MkPrefix pref i i'
-			        -> entails S I (x::G) i'
-					-> entails S I G result
+                    -> result:term
+                    -> pref:prefix
+                    -> MkPrefix pref (ForallT x i) result
+                    -> MkPrefix pref i i'
+                    -> entails S I (x::G) i'
+                    -> entails S I G result
 
   | Entails_Q_Inst : S:substrate -> I:infostrate -> G:varDecl
                    -> v:var
-				   -> i:term 
-				   -> i':term
-				   -> u:term
-				   -> pref:prefix
-				   -> hyp:term
-				   -> result:term
-				   -> MkPrefix pref (ForallT v i) hyp
+                   -> i:term
+                   -> i':term
+                   -> u:term
+                   -> pref:prefix
+                   -> hyp:term
+                   -> result:term
+                   -> MkPrefix pref (ForallT v i) hyp
                    -> Subst i v u i'
-				   -> MkPrefix pref i' result
-				   -> entails S I G hyp
-				   -> types G u v.typ
-				   -> entails S I G result
- 
+                   -> MkPrefix pref i' result
+                   -> entails S I G hyp
+                   -> types G u v.typ
+                   -> entails S I G result
+
   | Entails_Q_Inst : S:substrate -> I:infostrate -> G:varDecl
                    -> v:var
-				   -> i:term
-				   -> i':term
-				   -> u:term
-				   -> pref:prefix
-				   -> hyp:term
-				   -> result:term
-				   -> MkPrefix pref (ForallT v i) hyp
-				   -> MkPrefix pref i' result
+                   -> i:term
+                   -> i':term
+                   -> u:term
+                   -> pref:prefix
+                   -> hyp:term
+                   -> result:term
+                   -> MkPrefix pref (ForallT v i) hyp
+                   -> MkPrefix pref i' result
                    -> entails S I G hyp
-				   -> types G u v.typ
+                   -> types G u v.typ
                    -> Subst i v u i'
-				   -> entails S I G result
-				 
+                   -> entails S I G result
+
   | Entails_And_Intro : S:substrate -> I:infostrate -> G:varDecl
                      -> i:term -> i':term
-                     -> j:term -> j':term 
+                     -> j:term -> j':term
                      -> result:term
                      -> pref: prefix
                      -> MkPrefix pref (App AndInfon [i; j]) result
                      -> MkPrefix pref i i'
                      -> MkPrefix pref j j'
-                     -> entails S I G i' 
-                     -> entails S I G j' 
+                     -> entails S I G i'
+                     -> entails S I G j'
                      -> entails S I G result
 
   | Entails_And_Elim1 : S:substrate -> I:infostrate -> G:varDecl
                      -> i : term -> i': term
                      -> j : term
-                     -> pref : list term 
+                     -> pref : list term
                      -> hyp : term
                      -> MkPrefix pref (App AndInfon [i; j]) hyp
                      -> MkPrefix pref i i'
                      -> entails S I G hyp
                      -> entails S I G i'
-	 
+
   | Entails_And_Elim2 : S:substrate -> I:infostrate -> G:varDecl
                      -> i : term
                      -> j : term -> j': term
-                     -> pref : list term 
+                     -> pref : list term
                      -> hyp : term
                      -> MkPrefix pref (App AndInfon [i; j]) hyp
                      -> MkPrefix pref j j'
                      -> entails S I G hyp
                      -> entails S I G j'
-	 
-  | Entails_W_Imp_Intro : S:substrate -> I:infostrate -> G:varDecl 
+
+  | Entails_W_Imp_Intro : S:substrate -> I:infostrate -> G:varDecl
                       -> i:term
-                      -> j:term -> j':term 
+                      -> j:term -> j':term
                       -> result:term
                       -> pref: list term
                       -> MkPrefix pref j j'
                       -> MkPrefix pref (App ImpliesInfon [i; j]) result
-                      -> entails S I G j' 
+                      -> entails S I G j'
                       -> entails S I G result
-					  
+
   | Entails_Imp_Elim : S:substrate -> I:infostrate -> G:varDecl
-                     -> i : term -> i':term
-                     -> j : term -> j':term
-                     -> pref : list term 
-                     -> hyp : term
+                     -> i : term -> i':term (* = pref i *)
+                     -> j : term -> j':term (* = pref j *)
+                     -> pref : list term
+                     -> hyp : term (* = pref ( i => j ) *)
                      -> MkPrefix pref i i'
                      -> MkPrefix pref (App ImpliesInfon [i; j]) hyp
-                     -> MkPrefix pref i j'
-					 -> entails S I G i'
+                     -> MkPrefix pref j j'
+                     -> entails S I G i'
                      -> entails S I G hyp
                      -> entails S I G j'
 
-					 
 
-					 
+
+
 (*************************)
 (* Derivation algorithms *)
-(*************************) 
+(*************************)
 
 val doType: g:varDecl -> t:term -> option(ty:typ * (types g t ty))
 (* val doTypeList : g:varDecl -> terms:list term -> typs:list typ -> option (Zip term typ (types G)) *)
@@ -367,161 +379,179 @@ val doType: g:varDecl -> t:term -> option(ty:typ * (types g t ty))
 let rec doType g = function
   | Var v -> (match mem v g with (* TODO: change with new rules *)
                 | None -> None
-				| Some m -> Some((v.typ, Types_Var g v m)))
+                | Some m -> Some((v.typ, Types_Var g v m)))
   | Const TrueT -> Some((Boolean, Types_ConstTrueT g))
   | Const FalseT -> Some((Boolean, Types_ConstFalseT g))
-  | Const(PrincipalConstant p) -> 
+  | Const(PrincipalConstant p) ->
       Some((Principal,
             Types_ConstPrincipalConstant g p))
   | ForallT x i -> (match doType (x::g) i with
                      | None -> None
-                     | Some((Infon, pr)) -> 
+                     | Some((Infon, pr)) ->
                          Some((Infon, Types_ForallT g x i pr))
-					 | Some _ -> None)
+                     | Some _ -> None)
   | App EmptyInfon [] -> Some(Infon, Types_AppEmptyInfon g)
   | App AsInfon [(SubstrateQueryTerm q)] ->
       Some((Infon, Types_AppAsInfon g q))
   | App SaidInfon [p; i] ->
       (match (doType g p, doType g i) with
-	     | (Some((Principal, prp)), Some((Infon, pri))) ->
-		      Some((Infon, Types_AppSaidInfon g p i prp pri))
-		 | _ -> None)
+         | (Some((Principal, prp)), Some((Infon, pri))) ->
+              Some((Infon, Types_AppSaidInfon g p i prp pri))
+         | _ -> None)
   | App AndInfon [i; j] ->
       (match (doType g i, doType g j) with
-	     | (Some((Infon, pri)), Some((Infon, prj))) ->
-		      Some((Infon, Types_AppAndInfon g i j pri prj))
-		 | _ -> None)
+         | (Some((Infon, pri)), Some((Infon, prj))) ->
+              Some((Infon, Types_AppAndInfon g i j pri prj))
+         | _ -> None)
   | App ImpliesInfon [i; j] ->
       (match (doType g i, doType g j) with
-	     | (Some((Infon, pri)), Some((Infon, prj))) ->
-		      Some((Infon, Types_AppImpliesInfon g i j pri prj))
-		 | _ -> None)
+         | (Some((Infon, pri)), Some((Infon, prj))) ->
+              Some((Infon, Types_AppImpliesInfon g i j pri prj))
+         | _ -> None)
   | App JustifiedInfon [i; e] ->
       (match (doType g i, doType g e) with
-	     | (Some((Infon, pri)), Some((Evidence, pre))) ->
-		      Some((Infon, Types_AppJustifiedInfon g i e pri pre))
-		 | _ -> None)
-  | App (RelationInfon r) l -> 
+         | (Some((Infon, pri)), Some((Evidence, pre))) ->
+              Some((Infon, Types_AppJustifiedInfon g i e pri pre))
+         | _ -> None)
+  | App (RelationInfon r) l ->
        Some((Infon, Types_AppRelationInfon g r l))
   | _ -> None
 
 val subst: i:term -> x:var -> u:term -> (i':term * Subst i x u i')
-let rec subst i x u = 
+let rec subst i x u =
   match i with
     | Var y when x=y -> u, Subst_VarRepl x u
     | Var y -> Var y, Subst_VarIgnore y u x (* Rk: no need for a second when. Nice! *)
     | Const c -> Const c, Subst_Const x u c
     | ForallT y j when x=y ->
         ForallT y j, Subst_ForallTIgnore x j u
-	| ForallT y j ->
-	    let (j', pr) = subst j x u in
+    | ForallT y j ->
+        let (j', pr) = subst j x u in
           ForallT y j', Subst_ForallTRepl y j x u j' pr
     | App f [] -> (App f [], Subst_App0 f x u)
-	| App f [i] -> let (i', pri) = subst i x u in
-	                 App f [i'], Subst_App1 f x u i i' pri
+    | App f [i] -> let (i', pri) = subst i x u in
+                     App f [i'], Subst_App1 f x u i i' pri
     | App f [i; j] -> let (i', pri) = subst i x u in
-	                  let (j', prj) = subst j x u in
-	                    App f [i'; j'], Subst_App2 f x u i i' j j' pri prj
-	| SubstrateQueryTerm q ->
-	    SubstrateQueryTerm q, Subst_SubstrateQueryTerm q x u
+                      let (j', prj) = subst j x u in
+                        App f [i'; j'], Subst_App2 f x u i i' j j' pri prj
+    | SubstrateQueryTerm q ->
+        SubstrateQueryTerm q, Subst_SubstrateQueryTerm q x u
 
-(*		
+(*
 let term_apply (t:term) (s:substitution) : term =
   t (* TODO, see term.fst *)
 
-let entails_subst _S _I _G t s = 
-  entails _S _I _G (term_apply t s)		
-*)		
+let entails_subst _S _I _G t s =
+  entails _S _I _G (term_apply t s)
+*)
 val doDerive: S:substrate -> I:infostrate -> G:varDecl
              -> pref:prefix -> target:term
-			 -> option (target':term *
-                        MkPrefix pref target target' * 
-				        entails S I G target')
+             -> option (target':term *
+                        MkPrefix pref target target' *
+                        entails S I G target')
+						
 val tryDerive: S:substrate -> I:infostrate -> G:varDecl
              -> pref:prefix -> target:term
-             -> infon:term{Mem infon I}
-			 -> option (target':term *
-                        MkPrefix pref target target' * 
-					    entails S I G target')
-						
-let rec tryDerive _S _I _G pref target infon = 
+             -> infon:term 
+			 -> entails S I G infon
+             -> option (target':term *
+                        MkPrefix pref target target' *
+                        entails S I G target')
+
+(* tries to derive (pref target) using (infon); pr is a proof on infon *)
+let rec tryDerive _S _I _G pref target infon pr =
   match infon with
   (* NO! need to use substitutions *)
-  (*
+   (*
   | App SaidInfon [p; infon2] ->
       (match pref with
-	   | p2 :: tl when p = p2 ->
+       | p2 :: tl when p = p2 ->
           (match tryDerive _S _I _G tl target infon2 with
              | Some((target', m, e)) ->
-			      (*let (target'', m2) = mkPrefix tl target in*)
+                  (*let (target'', m2) = mkPrefix tl target in*)
                   Some((App SaidInfon [p; target'],
                         MkPrefix_Cons p tl target target' m,
                         e))
-			 | _ -> None)
-	   | _ -> None) *)(*
-  | App ImpliesInfon [i; j] ->
-      (match tryDerive _S _I _G pref target j with
-        | None -> None 
-        | Some((j', mj, ej)) ->
-        (match doDerive _S _I _G pref i with
-           | None -> None
-           | Some((i', mi, ei)) ->
-		       let (hyp, mhyp) = mkPrefix pref infon in
-               (b', mb,
-               Entails_Imp_Elim _S _I _G a a' b b' pref hyp ma mhyp mb ea 
-			     ) *)
-		
+             | _ -> None)
+       | _ -> None) *)
+  | App ImpliesInfon [i; j] -> (* to use i => j you need to *)
+      (match doDerive _S _I _G [] i with (* first prove i *)
+       | None -> None
+       | Some((i', mi, ei)) ->
+          let (j', mj) = mkPrefix [] j in
+          let (hyp, mhyp) = mkPrefix [] infon in 
+		  let prj = Entails_Imp_Elim _S _I _G i i' j j' [] hyp mi mhyp mj ei pr in
+            tryDerive _S _I _G pref target j prj) (* then prove (pref target) using j *)
+  | App AndInfon [i; j] -> (* to use i and j, we can either use i or use j *)
+	  let (hyp, mhyp) = mkPrefix [] infon in
+	  let (i', mi) = mkPrefix [] i in
+      (match tryDerive _S _I _G pref target i
+	          (Entails_And_Elim1 _S _I _G i i' j [] hyp mhyp mi pr) with
+	     | Some a -> Some a
+	     | None -> 
+		    (let (j', mj) = mkPrefix [] j in
+		     tryDerive _S _I _G pref target j
+			   (Entails_And_Elim2 _S _I _G i j j' [] hyp mhyp mj pr))) 
   | _ -> None
-						
-and doDerive _S _I _G pref target = 
+
+and doDerive _S _I _G pref target =
   let memInfostrate_target = memInfostrate target _I in
-  match target with 
+  match target with
   | App EmptyInfon [] -> let (j, m) = mkPrefix pref target in
-		              (* if unable to make F* prove sth, put in a runtime check *)
-			          (* if j = Empty then *)
-                   Some((j, m, 
-				         Entails_Emp _S _I _G pref j m))
-				      (* else raise "stupid F*" *)
+                      (* if unable to make F* prove sth, put in a runtime check *)
+                      (* if j = Empty then *)
+                     Some((j, m,
+                          Entails_Emp _S _I _G pref j m))
+                      (* else raise "stupid F*" *)
 
   | i when ((pref = []) && (not (memInfostrate_target = None))) ->
       let (j, m) = mkPrefix pref target in
-	  (match memInfostrate_target with
-	     | None -> raise "assert false"
+      (match memInfostrate_target with
+         | None -> raise "assert false"
          | Some mis -> Some((j, m, Entails_Hyp_Knowledge _S _I _G i mis)))
 
-  | App AsInfon [SubstrateQueryTerm q] ->  
-      (match pref with 
-         | [] -> let (j, m) = mkPrefix pref target in 
-             (match check_substrate _S q with  
-                | false -> None 
-                | true -> Some ((j, m, Entails_Hyp_Substrate _S _I _G q))) 
-         | _ -> None) 
-
+  | App AsInfon [SubstrateQueryTerm q] ->
+      (match pref with
+         | [] -> let (j, m) = mkPrefix pref target in
+             (match check_substrate _S q with
+                | false -> None
+                | true -> Some((j, m, Entails_Hyp_Substrate _S _I _G q)))
+         | _ -> None)
+		 
   | ForallT x i ->
       (match doDerive _S _I (x::_G) pref i with
-	     | None -> None
-		 | Some((i', mi, ei)) -> 
+         | None -> None
+         | Some((i', mi, ei)) ->
              let (j, m) = mkPrefix pref target in
-	         Some((j, m, Entails_Q_Intro _S _I _G x i i' j pref m mi ei)))
-	 
+                Some((j, m, Entails_Q_Intro _S _I _G x i i' j pref m mi ei)))
+
+  (*| ForallT x i -> 
+     map
+       (fun (i', mi, ei) ->
+           let (j, m) = mkPrefix pref target in
+              (j, m, Entails_Q_Intro _S _I _G x i i' j pref m mi ei))
+	   (doDerive _S _I (x::_G) pref i)*)
+
   | App AndInfon [i; j] -> (* TODO: extend to n variables *)
       (match (doDerive _S _I _G pref i, doDerive _S _I _G pref j) with
-	     | (None, _) -> None
-	     | (_, None) -> None
-	     | (Some((i', mi, ei)), Some((j', mj, ej))) -> 
-		      let (a, m) = mkPrefix pref target in
-		      Some((a, m,
+         | (None, _) -> None
+         | (_, None) -> None
+         | (Some((i', mi, ei)), Some((j', mj, ej))) ->
+              let (a, m) = mkPrefix pref target in
+              Some((a, m,
                     Entails_And_Intro _S _I _G i i' j j' a pref m mi mj ei ej)))
-					
+  
   | App ImpliesInfon [i; j] ->
       (match doDerive _S _I _G pref j with
-	     | None -> None
+         | None -> None
          | Some((j', mj, ej)) ->
              let (a, m) = mkPrefix pref target in
-			 Some((a, m,
-			       Entails_W_Imp_Intro _S _I _G i j j' a pref mj m ej)))
+             Some((a, m,
+                   Entails_W_Imp_Intro _S _I _G i j j' a pref mj m ej)))
 
-  (*| _ -> (* eventually, a collect; for now only pick the first one *)
-    fold_left (fun res infon -> match res with
-		         | None -> tryDerive _S _I _G pref target infon
-		         | _ -> res) None _I *)
+ (* | _ -> (* eventually, a collect; for now only pick the first one *)
+    fold_left_dep  None _I
+                   (fun res infon pr_mem -> match res with
+                      | None -> tryDerive _S _I _G pref target infon
+                                (Entails_Hyp_Knowledge _S _I _G infon pr_mem)
+                      | _ -> res) *)
